\documentclass[a4paper]{article}

\usepackage[utf8]{inputenc}
\usepackage{latexsym,amssymb,amsmath,amstext}
\usepackage{graphicx}
\usepackage[backend=bibtex, sorting=none]{biblatex}
\usepackage{subfigure}
\usepackage{float}

\bibliography{refs}

\begin{document}

\section{Model}

Based on the paper: \cite{axions_from_strings}.

\begin{equation}
    \mathcal{L} = - \frac{1}{2} ( \partial \phi )^2 + V(\phi)
\end{equation}

\begin{equation}
    V(\phi) = \frac{m_r^2}{2 f_a^2}\left( |\phi|^2 - \frac{f_a^2}{2} \right)^2
\end{equation}

\begin{equation}
    \phi(x) = \frac{r(x) + f_a}{\sqrt{2}} e^{i a(x) / f_a}
\end{equation}

\begin{equation}
    \varrho = T_{00} = \underbrace{\frac{1}{2} \dot{a}^2 + \frac{1}{2} | \nabla a|^2}_{= \varrho_\mathrm{axion}}
    + \underbrace{ \frac{1}{2} \dot{r}^2 + \frac{1}{2} | \nabla r|^2 + V(r) }_{= \varrho_\mathrm{radion}}
    + \left(\frac{r^2}{2 f_a^2} + \frac{r}{f_a} \right) (\dot{a}^2 + |\nabla a|^2)
\end{equation}

using the metric
\begin{equation}
    \mathrm{d}s^2 = -\mathrm{d}t^2 + a(t) \mathrm{d} x_i \mathrm{d} x_i
\end{equation}
and the Hubble parameter in the radiation domainted era ($\rho \sim a^{-4}$)
\begin{equation}
    H = \frac{1}{2t}
\end{equation}
$a$ is the scale factor obeying the Friedmann equation
\begin{equation}
    2 M_\mathrm{pl}^2 H^2 = \rho_\mathrm{total} = \frac{\pi^2}{30} g_* T^4
\end{equation}

Equation of Motion from the Lagragian:
\begin{equation}
    \ddot{\phi} + 3 H \dot{\phi} - \nabla^2 \phi + \phi \frac{m_r^2}{f_a^2} \left( |\phi|^2 - \frac{f_a^2}{2} \right) = 0
\end{equation}

\begin{equation}
    \ddot{\phi} + 3 H \dot{\phi} - \nabla^2 \phi + \phi m_r^2 \left( \frac{|\phi|^2}{f_a^2} - \frac{1}{2} \right) = 0
\end{equation}

Divide by $m_r^2$ and $f_a$:
\begin{equation}
    \frac{\mathrm{d}^2 {\phi}}{\mathrm{d} t^2 f_a m_r^2} + 3 \frac{H}{m_r} \frac{\mathrm{d} \phi}{\mathrm{d} t m_r f_a} - \frac{\nabla^2 \phi}{m_r^2 f_a} + \frac{\phi}{f_a} \left( \frac{ |\phi|^2 } { f_a^2 } - \frac{1}{2} \right) = 0
\end{equation}

Using the replacements:
\begin{align}
    t' &= m_r t \\
    H' &= H / m_r \\
    x' &= m_r x \\
    \phi' &= \phi / f_a
\end{align}

we find:
\begin{equation}
    \frac{\mathrm{d}^2 \phi'}{\mathrm{d} t'^2} + 3 H' \frac{\mathrm{d} \phi'}{\mathrm{d} t'} - \nabla'^2 \phi + \phi' \left( |\phi'|^2 - \frac{1}{2} \right) = 0
\end{equation}

\begin{equation}
    \phi'(x') = \frac{r(x)/f_a + 1}{\sqrt{2}} e^{i a(x) / f_a}
\end{equation}

Define the conformal time $\tau$ such that:
\begin{equation}
    \frac{\mathrm{d} \tau}{\mathrm{d} t} = \frac{1}{a(t)}
\end{equation}
hence:
\begin{equation}
    \frac{\mathrm{d}}{\mathrm{d} t} = \frac{\mathrm{d \tau}}{\mathrm{d} t} \frac{\mathrm{d}}{\mathrm{d} \tau} = \frac{1}{a(t)} \frac{\mathrm{d}}{\mathrm{d} \tau}
\end{equation}

\begin{align}
    \frac{\mathrm{d}^2}{\mathrm{d} t^2} = \frac{\mathrm{d}}{\mathrm{d} t} \frac{1}{a} \frac{\mathrm{d}}{\mathrm{d} \tau}
    = - \frac{\dot{a}}{a^2} \frac{\mathrm{d}}{\mathrm{d} \tau} + \frac{1}{a} \frac{\mathrm{d}}{\mathrm{d} t} \frac{\mathrm{d}}{\mathrm{d} \tau}
     = - \frac{\dot{a}}{a^2} \frac{\mathrm{d}}{\mathrm{d} \tau} + \frac{1}{a^2} \frac{\mathrm{d}^2}{\mathrm{d} \tau^2}
\end{align}

where
\begin{equation}
    \frac{\mathrm{d} 1/a}{\mathrm{d} \tau} = - a' / a^2 = - a \dot{a} / a^2 = - H
\end{equation}

Now use unprimed quantities and use the prime as the derivative with respect to $\tau$.
\begin{equation}
    - 1/a H \phi' + 1/a^2 \phi'' + 3 H / a \phi'
    - \nabla^2 \phi + \phi \left( |\phi|^2 - \frac{1}{2} \right) = 0
\end{equation}

\begin{equation}
    \frac{\mathrm{d} a(t)}{\mathrm{d} \tau} = \frac{\mathrm{d} t}{\mathrm{d} \tau} \dot{a} = \dot{a} / \frac{\mathrm{d} \tau}{\mathrm{d} t} = \dot{a} / (1 / a(t)) = \dot{a} a
\end{equation}

\begin{equation}
    \phi = \psi / a
\end{equation}

\begin{equation}
    \frac{\mathrm{d}}{\mathrm{d} \tau} ( \psi / a(t) ) = \frac{\mathrm{d} \psi}{\mathrm{d} \tau} / a(t) - \frac{\mathrm{d} a(t)}{\mathrm{d} \tau} \psi / a^2(t)
    = \frac{\mathrm{d} \psi}{\mathrm{d} \tau} / a(t) - \dot{a} a \psi / a^2(t)
    = \psi' / a - \psi H
\end{equation}

\begin{equation}
    \frac{d H}{d \tau} = \frac{d t}{d \tau} \frac{d H}{d t} = a (\ddot{a} / a - \dot{a}^2 / a^2) = \ddot{a} - a H^2
\end{equation}

\begin{equation}
    \frac{d^2}{d \tau^2} (\psi / a) = \frac{d}{d \tau} (\psi' / a - \psi H)
    = \psi'' / a - \psi' H - (\psi' H + \psi \frac{d H}{d \tau})
    = \psi'' / a - 2 \psi' H - \psi ( \ddot{a} - a H^2 )
\end{equation}

\begin{equation}
    1/a^2 ( \psi'' / a - 2 \psi' H - \psi ( \ddot{a} - a H^2 ) ) + 2 H / a (\psi' / a - \psi H)
    - \nabla^2 \psi / a + \psi / a \left( |\psi / a|^2 - \frac{1}{2} \right) = 0
\end{equation}

\begin{equation}
    \psi'' / a^3 - 2 \psi' H / a^2 - \psi \ddot{a} / a^2 + \psi H^2 / a
    + 2 \psi' H / a^2 - 2 H^2 \psi / a
    - \nabla^2 \psi / a + \psi / a^3 ( |\psi|^2 - \frac{a^2}{2} ) = 0
\end{equation}

\begin{equation}
    \psi'' / a^3 - \psi \ddot{a} / a^2 - H^2 \psi / a
    - \nabla^2 \psi / a + \psi / a^3 ( |\psi|^2 - \frac{a^2}{2} ) = 0
\end{equation}

\begin{equation}
    \psi'' + \psi (\underbrace{- \ddot{a} a - H^2 a^2}_{= 0})
    - \nabla^2 \psi a^2 + \psi ( |\psi|^2 - \frac{a^2}{2} ) = 0
\end{equation}

\begin{equation}
    \tilde{x} = x' / a
\end{equation}

\begin{equation}
    \psi'' - \tilde{\nabla}^2 \psi + \psi ( |\psi|^2 - \frac{a^2}{2} ) = 0
\end{equation}

\begin{equation}
    a = a_1 t^{1/2}
\end{equation}
\begin{equation}
    H = \frac{1}{2t}
\end{equation}

\begin{equation}
    \tau(t) = \int_0^t \mathrm{d} t' a^{-1}(t') = \int_0^t \mathrm{d} t' a_1 t^{-1/2} = -2 a_1 t^{1/2}
\end{equation}


\newpage
\printbibliography

\end{document}
